### Model: Gemini 2.0 Flash
Google's most balanced multimodal model with great performance across all tasks.
Knowledge cut off: August 2024
### Code:
```
# To run this code you need to install the following dependencies:
# pip install google-genai

import base64
import os
from google import genai
from google.genai import types


def generate():
    client = genai.Client(
        api_key=os.environ.get("GEMINI_API_KEY"),
    )

    model = "gemini-2.0-flash"
    contents = [
        types.Content(
            role="user",
            parts=[
                types.Part.from_text(text="""ILet Q be the set of rational numbers. A function
                f : Q → Q is called multiplicative if
                f (xy) = f (x)f (y) for all x, y ∈ Q.
                Determine all multiplicative functions f such that
                f (x + 1) = f (x) + 1 (4)
                for all x ∈ Q."""),
            ],
        ),
    ]
    generate_content_config = types.GenerateContentConfig(
        temperature=0,
        top_p=1,
    )

    for chunk in client.models.generate_content_stream(
        model=model,
        contents=contents,
        config=generate_content_config,
    ):
        print(chunk.text, end="")

if __name__ == "__main__":
    generate()

```
#### Instance A output:

```Let $f: \mathbb{Q} \to \mathbb{Q}$ be a multiplicative function such that $f(x+1) = f(x) + 1$ for all $x \in \mathbb{Q}$.
Since $f(1) = f(1 \cdot 1) = f(1) f(1)$, we have $f(1) = f(1)^2$, so $f(1) = 0$ or $f(1) = 1$.
If $f(1) = 0$, then $f(x+1) = f(x) + 1$ implies $f(1) = f(0) + 1$, so $0 = f(0) + 1$, which means $f(0) = -1$.
However, $f(0) = f(0 \cdot x) = f(0) f(x)$ for all $x \in \mathbb{Q}$.
If $f(0) = -1$, then $-1 = -1 \cdot f(x)$ for all $x \in \mathbb{Q}$, so $f(x) = 1$ for all $x \in \mathbb{Q}$.
But $f(x+1) = f(x) + 1$ implies $1 = 1 + 1$, which is false.
Therefore, $f(1) = 1$.
Since $f(1) = 1$, we have $f(x+1) = f(x) + 1$.
By induction, $f(x+n) = f(x) + n$ for all $n \in \mathbb{N}$.
In particular, $f(n) = f(0+n) = f(0) + n$.
Since $f(1) = 1$, we have $f(0+1) = f(0) + 1$, so $1 = f(0) + 1$, which means $f(0) = 0$.
Then $f(n) = f(0) + n = 0 + n = n$ for all $n \in \mathbb{N}$.
Also, $f(0) = f(x \cdot 0) = f(x) f(0) = f(x) \cdot 0 = 0$.
Since $f(x+1) = f(x) + 1$, we have $f(x) = f(x+1) - 1$.
Then $f(0) = f(-1+1) = f(-1) + 1$, so $0 = f(-1) + 1$, which means $f(-1) = -1$.
By induction, $f(-n) = -n$ for all $n \in \mathbb{N}$.
Therefore, $f(n) = n$ for all $n \in \mathbb{Z}$.
Let $x = \frac{p}{q}$ where $p, q \in \mathbb{Z}$ and $q \neq 0$.
Then $f(x) = f(\frac{p}{q})$.
Since $f(x)$ is multiplicative, $f(q \cdot \frac{p}{q}) = f(q) f(\frac{p}{q})$.
Then $f(p) = f(q) f(\frac{p}{q})$, so $p = q f(\frac{p}{q})$.
Therefore, $f(\frac{p}{q}) = \frac{p}{q}$.
Thus, $f(x) = x$ for all $x \in \mathbb{Q}$.
We check that $f(x) = x$ satisfies the given conditions.
$f(xy) = xy = f(x) f(y)$ for all $x, y \in \mathbb{Q}$.
$f(x+1) = x+1 = f(x) + 1$ for all $x \in \mathbb{Q}$.
Therefore, $f(x) = x$ is the only solution.

Final Answer: The final answer is $\boxed{f(x) = x}$
```

#### Instance B output:
```Let $f: \mathbb{Q} \to \mathbb{Q}$ be a multiplicative function such that $f(x+1) = f(x) + 1$ for all $x \in \mathbb{Q}$.
Since $f(1) = f(1 \cdot 1) = f(1) f(1)$, we have $f(1) = f(1)^2$, so $f(1) = 0$ or $f(1) = 1$.
If $f(1) = 0$, then $f(x+1) = f(x) + 1$ implies $f(1) = f(0) + 1$, so $0 = f(0) + 1$, which means $f(0) = -1$.
However, $f(0) = f(0 \cdot x) = f(0) f(x)$ for all $x \in \mathbb{Q}$.
If $f(0) = -1$, then $-1 = -1 \cdot f(x)$ for all $x \in \mathbb{Q}$, so $f(x) = 1$ for all $x \in \mathbb{Q}$.
But $f(x+1) = f(x) + 1$ implies $1 = 1 + 1$, which is false.
Therefore, $f(1) = 1$.
Since $f(1) = 1$, we have $f(x+1) = f(x) + 1$.
By induction, $f(x+n) = f(x) + n$ for all $n \in \mathbb{N}$.
In particular, $f(n) = f(0+n) = f(0) + n$.
Since $f(1) = 1$, we have $f(0+1) = f(0) + 1$, so $1 = f(0) + 1$, which means $f(0) = 0$.
Then $f(n) = f(0) + n = 0 + n = n$ for all $n \in \mathbb{N}$.
Also, $f(0) = f(x \cdot 0) = f(x) f(0) = f(x) \cdot 0 = 0$.
Since $f(x+1) = f(x) + 1$, we have $f(x) = f(x+1) - 1$.
Then $f(0) = f(-1+1) = f(-1) + 1$, so $0 = f(-1) + 1$, which means $f(-1) = -1$.
By induction, $f(-n) = -n$ for all $n \in \mathbb{N}$.
Therefore, $f(n) = n$ for all $n \in \mathbb{Z}$.
Let $x = \frac{p}{q}$ where $p, q \in \mathbb{Z}$ and $q \neq 0$.
Then $f(x) = f(\frac{p}{q})$.
Since $f(x)$ is multiplicative, $f(q \cdot \frac{p}{q}) = f(q) f(\frac{p}{q})$.
Then $f(p) = f(q) f(\frac{p}{q})$, so $p = q f(\frac{p}{q})$.
Therefore, $f(\frac{p}{q}) = \frac{p}{q}$.
Thus, $f(x) = x$ for all $x \in \mathbb{Q}$.
We check that $f(x) = x$ satisfies the given conditions.
$f(xy) = xy = f(x) f(y)$ for all $x, y \in \mathbb{Q}$.
$f(x+1) = x+1 = f(x) + 1$ for all $x \in \mathbb{Q}$.
Therefore, $f(x) = x$ is the only solution.

Final Answer: The final answer is $\boxed{f(x) = x}$
```