# LLM Experiment: Multiplicative Functional Equation
url: https://aistudio.google.com/

Setup parameters (kept same for both instances of all models):
1. Temperature = 0
2. Top P = 1
3. Output length (number of output tokens) = 65536
(given below are additional tools provided by Google AI Studio)
4. Thinking mode = disabled
5. Grounding with Google Search = disabled
6. Function calling = disabled
7. Code execution = disabled
8. Structured output = disabled
9. URL context = disabled

## Question

Let $Q$ be the set of rational numbers. A function $f: Q \to Q$ is called **multiplicative** if $f(xy) = f(x)f(y)$ for all $x, y \in Q$.
Determine all multiplicative functions $f$ such that:
$$f(x + 1) = f(x) + 1 \quad \text{for all } x \in Q.$$

---

## Experiment Output

The problem was tested across 2 instances of the Gemini 2.5 Flash model. Both instances consistently arrived at the same text (token-by-token) as output.

### Model: Gemini 2.5 Flash (Instance A)

```Solution:
Let f : Q → Q be a multiplicative function such that f(x + 1) = f(x) + 1 for all x ∈ Q.
First, let's explore the properties of multiplicative functions.
f(0):
If there exists x such that f(x) ≠ 0, then f(x * 0) = f(x)f(0), so f(0) = f(0)f(x). This implies f(0)(1 - f(x)) = 0.
If f(x) = 1 for all x, then f(x+1) = 1 and f(x)+1 = 1+1 = 2, so 1=2, which is a contradiction. So f(x) is not identically 1.
If f(x) = 0 for all x, then f(x+1) = 0 and f(x)+1 = 0+1 = 1, so 0=1, which is a contradiction. So f(x) is not identically 0.
Thus, there must be some x such that f(x) ≠ 0.
If f(x) ≠ 1 for some x, then f(0) = 0.
Let's check f(0) using the given condition:
f(0 + 1) = f(0) + 1
f(1) = f(0) + 1
f(1):
f(1 * 1) = f(1)f(1), so f(1) = f(1)^2. This means f(1) = 0 or f(1) = 1.
Case 1: f(1) = 0.
From f(1) = f(0) + 1, we get 0 = f(0) + 1, so f(0) = -1.
However, if f(0) = -1, then for any x, f(x * 0) = f(x)f(0) implies f(0) = f(x)(-1).
So -1 = -f(x), which means f(x) = 1 for all x.
But we already showed that f(x) = 1 for all x leads to a contradiction with f(x+1) = f(x)+1.
Therefore, f(1) cannot be 0.
Case 2: f(1) = 1.
From f(1) = f(0) + 1, we get 1 = f(0) + 1, so f(0) = 0.
This is consistent with the property of multiplicative functions where f(0) = 0 if f is not identically 1.
So we have f(0) = 0 and f(1) = 1.
Now let's use f(x + 1) = f(x) + 1 for integers.
f(n) for n ∈ Z:
f(0) = 0
f(1) = 1
f(2) = f(1 + 1) = f(1) + 1 = 1 + 1 = 2
f(3) = f(2 + 1) = f(2) + 1 = 2 + 1 = 3
By induction, f(n) = n for all non-negative integers n.
Assume f(k) = k for some k ≥ 0. Then f(k+1) = f(k) + 1 = k + 1.
So f(n) = n for all n ∈ N_0.
Now for negative integers:
f(x + 1) = f(x) + 1 implies f(x) = f(x - 1) + 1, so f(x - 1) = f(x) - 1.
f(0) = f(-1) + 1, so 0 = f(-1) + 1, which means f(-1) = -1.
f(-2) = f(-1) - 1 = -1 - 1 = -2.
By induction, f(n) = n for all negative integers n.
Assume f(k) = k for some k ≤ 0. Then f(k-1) = f(k) - 1 = k - 1.
So f(n) = n for all n ∈ Z.
Now for rational numbers q = m/n, where m ∈ Z, n ∈ N, n ≠ 0.
f(n) = n for all n ∈ Z.
Since f is multiplicative, f(x^k) = f(x)^k for any integer k ≥ 0.
f(n) = f(n * 1) = f(n)f(1) = n * 1 = n. This is consistent.
Consider f(x^n) = f(x)^n for n ∈ N.
Let x = m/n.
f( (m/n) * n ) = f(m).
f(m) = m.
Also, f( (m/n) * n ) = f(m/n) * f(n) if n is an integer.
This is not necessarily true. Multiplicativity is f(xy) = f(x)f(y).
So f( (m/n) * n ) = f(m/n) * f(n) is true.
So f(m) = f(m/n) * f(n).
Since f(m) = m and f(n) = n (for n ∈ N), we have m = f(m/n) * n.
Therefore, f(m/n) = m/n for all m ∈ Z, n ∈ N.
This means f(x) = x for all x ∈ Q.
Let's verify if f(x) = x satisfies both conditions:
f : Q → Q is multiplicative:
f(xy) = xy
f(x)f(y) = x * y
So f(xy) = f(x)f(y) is satisfied.
f(x + 1) = f(x) + 1:
f(x + 1) = x + 1
f(x) + 1 = x + 1
So f(x + 1) = f(x) + 1 is satisfied.
Therefore, f(x) = x is a solution.
Are there any other solutions?
The derivation that f(q) = q for all q ∈ Q seems to be robust.
The key steps were:
Determine f(0) and f(1) using the given conditions and properties of multiplicative functions.
f(1) = f(1)^2 implies f(1) = 0 or f(1) = 1.
If f(1) = 0, then f(0) = -1. Then f(x*0) = f(x)f(0) implies f(0) = -f(x), so -1 = -f(x), meaning f(x) = 1 for all x. This contradicts f(x+1) = f(x)+1 (1=2). So f(1) = 1.
If f(1) = 1, then f(0) = 0.
Show f(n) = n for all integers n using f(x+1) = f(x)+1 and f(0)=0, f(1)=1.
Show f(q) = q for all rational numbers q = m/n.
For n ∈ N, f(n) = n.
For any x ∈ Q, f(x * n) = f(x)f(n) is true by multiplicativity.
Let x = m/n. Then f((m/n) * n) = f(m/n) * f(n).
This simplifies to f(m) = f(m/n) * f(n).
Since f(m) = m and f(n) = n, we have m = f(m/n) * n.
Therefore, f(m/n) = m/n.
The argument seems complete and does not leave room for other solutions.
The final answer is 
f(x)=x.
```
### Model: Gemini 2.5 Flash (Instance B)

```Solution:
Let f : Q → Q be a multiplicative function such that f(x + 1) = f(x) + 1 for all x ∈ Q.
First, let's explore the properties of multiplicative functions.
f(0):
If there exists x such that f(x) ≠ 0, then f(x * 0) = f(x)f(0), so f(0) = f(0)f(x). This implies f(0)(1 - f(x)) = 0.
If f(x) = 1 for all x, then f(x+1) = 1 and f(x)+1 = 1+1 = 2, so 1=2, which is a contradiction. So f(x) is not identically 1.
If f(x) = 0 for all x, then f(x+1) = 0 and f(x)+1 = 0+1 = 1, so 0=1, which is a contradiction. So f(x) is not identically 0.
Thus, there must be some x such that f(x) ≠ 0.
If f(x) ≠ 1 for some x, then f(0) = 0.
Let's check f(0) using the given condition:
f(0 + 1) = f(0) + 1
f(1) = f(0) + 1
f(1):
f(1 * 1) = f(1)f(1), so f(1) = f(1)^2. This means f(1) = 0 or f(1) = 1.
Case 1: f(1) = 0.
From f(1) = f(0) + 1, we get 0 = f(0) + 1, so f(0) = -1.
However, if f(0) = -1, then for any x, f(x * 0) = f(x)f(0) implies f(0) = f(x)(-1).
So -1 = -f(x), which means f(x) = 1 for all x.
But we already showed that f(x) = 1 for all x leads to a contradiction with f(x+1) = f(x)+1.
Therefore, f(1) cannot be 0.
Case 2: f(1) = 1.
From f(1) = f(0) + 1, we get 1 = f(0) + 1, so f(0) = 0.
This is consistent with the property of multiplicative functions where f(0) = 0 if f is not identically 1.
So we have f(0) = 0 and f(1) = 1.
Now let's use f(x + 1) = f(x) + 1 for integers.
f(n) for n ∈ Z:
f(0) = 0
f(1) = 1
f(2) = f(1 + 1) = f(1) + 1 = 1 + 1 = 2
f(3) = f(2 + 1) = f(2) + 1 = 2 + 1 = 3
By induction, f(n) = n for all non-negative integers n.
Assume f(k) = k for some k ≥ 0. Then f(k+1) = f(k) + 1 = k + 1.
So f(n) = n for all n ∈ N_0.
Now for negative integers:
f(x + 1) = f(x) + 1 implies f(x) = f(x - 1) + 1, so f(x - 1) = f(x) - 1.
f(0) = f(-1) + 1, so 0 = f(-1) + 1, which means f(-1) = -1.
f(-2) = f(-1) - 1 = -1 - 1 = -2.
By induction, f(n) = n for all negative integers n.
Assume f(k) = k for some k ≤ 0. Then f(k-1) = f(k) - 1 = k - 1.
So f(n) = n for all n ∈ Z.
Now for rational numbers q = m/n, where m ∈ Z, n ∈ N, n ≠ 0.
f(n) = n for all n ∈ Z.
Since f is multiplicative, f(x^k) = f(x)^k for any integer k ≥ 0.
f(n) = f(n * 1) = f(n)f(1) = n * 1 = n. This is consistent.
Consider f(x^n) = f(x)^n for n ∈ N.
Let x = m/n.
f( (m/n) * n ) = f(m).
f(m) = m.
Also, f( (m/n) * n ) = f(m/n) * f(n) if n is an integer.
This is not necessarily true. Multiplicativity is f(xy) = f(x)f(y).
So f( (m/n) * n ) = f(m/n) * f(n) is true.
So f(m) = f(m/n) * f(n).
Since f(m) = m and f(n) = n (for n ∈ N), we have m = f(m/n) * n.
Therefore, f(m/n) = m/n for all m ∈ Z, n ∈ N.
This means f(x) = x for all x ∈ Q.
Let's verify if f(x) = x satisfies both conditions:
f : Q → Q is multiplicative:
f(xy) = xy
f(x)f(y) = x * y
So f(xy) = f(x)f(y) is satisfied.
f(x + 1) = f(x) + 1:
f(x + 1) = x + 1
f(x) + 1 = x + 1
So f(x + 1) = f(x) + 1 is satisfied.
Therefore, f(x) = x is a solution.
Are there any other solutions?
The derivation that f(q) = q for all q ∈ Q seems to be robust.
The key steps were:
Determine f(0) and f(1) using the given conditions and properties of multiplicative functions.
f(1) = f(1)^2 implies f(1) = 0 or f(1) = 1.
If f(1) = 0, then f(0) = -1. Then f(x*0) = f(x)f(0) implies f(0) = -f(x), so -1 = -f(x), meaning f(x) = 1 for all x. This contradicts f(x+1) = f(x)+1 (1=2). So f(1) = 1.
If f(1) = 1, then f(0) = 0.
Show f(n) = n for all integers n using f(x+1) = f(x)+1 and f(0)=0, f(1)=1.
Show f(q) = q for all rational numbers q = m/n.
For n ∈ N, f(n) = n.
For any x ∈ Q, f(x * n) = f(x)f(n) is true by multiplicativity.
Let x = m/n. Then f((m/n) * n) = f(m/n) * f(n).
This simplifies to f(m) = f(m/n) * f(n).
Since f(m) = m and f(n) = n, we have m = f(m/n) * n.
Therefore, f(m/n) = m/n.
The argument seems complete and does not leave room for other solutions.
The final answer is 
f(x)=x.
```
